Core.lean
@@ -1,3 +1,4 @@
 import Core.Examples
 import Core.Infer
 import Core.Metatheory
+import Core.Eval
